\section{Approximate Analytical Policy Efficiency Ratio}
\label{app:cer}
Using an approximation from \cite{bartmann1992inventory}
\begin{equation}
	\frac{\Gamma(x,y)}{\Gamma(x)}\simeq \frac{1}{1+e^{-\frac{m}{\sqrt{y}}(x-y-\frac{1}{2})}}
\end{equation}
with $m\simeq 1.8$. Applying this yields
\begin{equation}
	\begin{split}
		\sum_{\zeta_t=0}^\infty1_{N_t> 0}p(\zeta_t| D, I) & \simeq \frac{1}{1+e^{-\frac{m}{\sqrt{\lambda_t}}(N_0+\upsilon_t+\frac{1}{2}-\lambda_t)}},\\
		\sum_{\zeta_t=0}^\infty1_{N_t> 0}\zeta_tp(\zeta_t| D, I) & \simeq \lambda_t\frac{1}{1+e^{-\frac{m}{\sqrt{\lambda_t}}(N_0+\upsilon_t-\frac{1}{2}-\lambda_t)}}.
	\end{split}
	\label{eq:hest}
\end{equation}
The expected cost of equation \eqref{eq:exact} can thus be written
\begin{equation}
	\begin{split}
		\mathbb{E}[C|D,I] \simeq \sum_{t=1}^{T} \gamma_{\text{disc}}^{t-1} \chi_t.
	\end{split}
\end{equation}
where for brevity
\begin{equation}
	\begin{split}
		\chi (\upsilon_t)\equiv 
		\frac{(h_t+c_t)(N_0 + \upsilon_t)}{1+e^{-\frac{m}{\sqrt{\lambda_t}}(N_0+\upsilon_t+\frac{1}{2}-\lambda_t)}}- \frac{(h_t+c_t)\lambda_t}{1+e^{-\frac{m}{\sqrt{\lambda_t}}(N_0+\upsilon_t-\frac{1}{2}-\lambda_t)}} - c_t(N_0 + \upsilon_t-\lambda_t)
	\end{split}
\end{equation}
and due to the lead time, legacy decisions for $t<0$ make up the expected cost for $t\in [1,L-1]$. 

\subsection{Optimal Expected Cost}
Combining equations \eqref{eq:hest}, \eqref{eq:hest2} and theorem \ref{theorem:opt_policy}, given that $t\geq L$ and $\upsilon_t^*\geq 0$, the optimal policy can be represented by
\begin{equation}
	\frac{c_t}{c_t+h_t}\simeq\frac{1}{1+e^{-\frac{m}{\sqrt{\lambda_t}}(N_0+\upsilon_t^*+\frac{1}{2}-\lambda_t)}}
\end{equation}
meaning
\begin{equation}
	\upsilon_t^* \simeq \max(\text{round}(\lambda_t+\frac{\sqrt{\lambda_t}}{m}\ln\frac{c_t}{h_t}-N_0-\frac{1}{2}),0)
\end{equation}
for $t\geq L$, yielding the optimal expected cost
\begin{equation}
	\begin{split}
		\mathbb{E}[C|D,I]\big|_{\pi=\pi^*} &\simeq \sum_{t=1}^{K^*-1}\gamma_{\text{disc}}^{t-1}\chi(\upsilon_t)+ \sum_{t=K^*}^{T} \gamma_{\text{disc}}^{t-1} \chi(\upsilon_t^*)\\
		&= E_{K^*}+\sum_{t=K^*}^{T} \gamma_{\text{disc}}^{t-1} \lambda_th_t\frac{e^{\frac{m}{\sqrt{\lambda_t}}}-1}{e^{\frac{m}{\sqrt{\lambda_t}}}\frac{h_t}{c_t}+1}.\\
	\end{split}
	\label{eq:opt_cost}
\end{equation}
where
\begin{equation}
	E_{K^*}\equiv \sum_{t=1}^{K^*-1}\gamma_{\text{disc}}^{t-1}\chi(\upsilon_t)
\end{equation}
and $L\leq K^* \leq T$ represent the time step where the fist decision is made based on the optimal policy (before this legacy decision can be made).

\subsection{Baseline Expected Cost}
Combining equation \eqref{eq:hest2} and definition \ref{def:baseline}
\begin{equation}  
	\upsilon_t' = \max(\text{round}(\lambda_t + R - N_0), 0), 
\end{equation} 
yielding
\begin{equation}
	\begin{split}
		\mathbb{E}[C|D,I]|_{\pi = \pi'} &\simeq \sum_{t=1}^{K'-1}\gamma_{\text{disc}}^{t-1}\chi(\upsilon_t)+\sum_{t=K'}^{T} \gamma_{\text{disc}}^{t-1} \chi(\upsilon_t')\\
		&\simeq E_{K'}+\sum_{t=K'}^{T} \gamma_{\text{disc}}^{t-1} \chi(\upsilon_t')\\
	\end{split}
	\label{eq:bas_cost}
\end{equation}
with
\begin{equation}
	\chi(\upsilon_t') = 
	\frac{(h_t+c_t)(\lambda_t+R)}{1+e^{-\frac{m}{\sqrt{\lambda_t}}(R+1)}}- \frac{(h_t+c_t)\lambda_t}{1+e^{-\frac{m}{\sqrt{\lambda_t}}R}} - c_tR.
\end{equation}

\subsection{Policy Efficiency Ratio}
Combining equation \eqref{eq:opt_cost} and \eqref{eq:bas_cost}
\begin{equation}
	\frac{\mathbb{E}[C|D,I]|_{\pi = \pi^*} }{\mathbb{E}[C|D,I]|_{\pi = \pi'}}\simeq \frac{E_{K^*}+\sum_{t=K^*}^{T} \gamma_{\text{disc}}^{t-1} \lambda_th_t\frac{e^{\frac{m}{\sqrt{\lambda_t}}}-1}{e^{\frac{m}{\sqrt{\lambda_t}}}\frac{h_t}{c_t}+1}}{E_{K'}+\sum_{t=K'}^{T} \gamma_{\text{disc}}^{t-1}h_t \bigg( 
		\frac{(1+\frac{c_t}{h_t})(\lambda_t+R)}{1+e^{-\frac{m}{\sqrt{\lambda_t}}(R+1)}}- \frac{(1+\frac{c_t}{h_t})\lambda_t}{1+e^{-\frac{m}{\sqrt{\lambda_t}}R}} - \frac{c_t}{h_t}R\bigg)}.
	\label{eq:per1}
\end{equation}
In order to further reduce equation \eqref{eq:per1} simplifying assumptions must be made.
\begin{axiom}[No legacy decisions]
	\label{ax:leg}
	 No legacy conditions mean $\upsilon_t=0$ for $t\in [1,L-1]$.
\end{axiom}
\begin{axiom}[Constant holding cost and unit value]
	\label{ax:const}
	Constant holding cost and unit value means $c_t=c$ and $h_t=h$ are independent of time.
\end{axiom}
\begin{axiom}[Significant demand]
	\label{ax:demand}
	Demand is significant if $\lambda_t\gg 0$.
\end{axiom}

\begin{axiom}[Constant demand]
	\label{ax:const_demand}
	Assuming constant demand means $\lambda_t=t\lambda$, where $\lambda >0$.
\end{axiom}

\begin{axiom}[Sufficient initial stock]
	\label{ax:initial_stock}
	Sufficient initial stock is defined such that $\lambda_{L-1} + R < N_0\ll \lambda_T$.
\end{axiom}

\begin{axiom}[Short lead time]
	Let $L\ll T$.
\end{axiom}

Using axiom \ref{ax:demand}
\begin{equation}
	1\leq e^{\frac{m}{\sqrt{\lambda_t}}}\lesssim 1.5 \Rightarrow  e^{\frac{m}{\sqrt{\lambda_t}}}\approx k
	\label{eq:k}
\end{equation}


Using axioms \ref{ax:const}, \ref{ax:leg} and \ref{ax:initial_stock} alongside equation \eqref{eq:k}
\begin{equation}
	\begin{split}
		\chi(\upsilon_t^*)&\approx \lambda_th\frac{k-1}{k\frac{h}{c}+1},\\
		\chi(\upsilon_t')|_{R\sim 0} &\simeq \frac{\lambda_t(h+c)}{2}
		\frac{e^{\frac{m}{\sqrt{\lambda_t}}}-1}{e^{\frac{m}{\sqrt{\lambda_t}}}+1}\\
		&\approx \frac{\lambda_th}{2}(1+\frac{c}{h})\frac{k-1}{k+1},\\
		\chi(\upsilon_t')|_{R\gg 0} &\approx hR,\\
		\chi(\upsilon_t)|_{t<L}&\approx h(N_0-\lambda_t)
	\end{split}
	\label{eq:ape}
\end{equation}
Assuming $\frac{m}{\sqrt{\lambda_t}}\ll 1$ for $\upsilon_t'$ and $\upsilon_t^*$, then
\begin{equation}
	\begin{split}
		\chi(\upsilon_t^*)&\sim \sqrt{\lambda_t}mh\frac{1}{\frac{h}{c}+1},\\
		\chi(\upsilon_t')|_{R\sim 0} &\sim \frac{\sqrt{\lambda_t}mh}{4}(1+\frac{c}{h}),\\
	\end{split}
\end{equation}
Combining equation \eqref{eq:ape} and \eqref{eq:per1} and taking $\gamma_{\text{disc}}=1$ and let $r= \frac{c}{h}$

\begin{equation}
	\frac{\mathbb{E}[C|D,I]|_{\pi = \pi^*} }{\mathbb{E}[C|D,I]|_{\pi = \pi'}}\bigg|_{R\sim 0}\sim \frac{\sum_{t=1}^{K^*-1}(N_0-\lambda_t)+m\frac{r}{r+1}\sum_{t=K^*}^{T}\sqrt{\lambda_t}}{\sum_{t=1}^{K'-1}(N_0-\lambda_t)+\frac{m}{4}(1+r)\sum_{t=K'}^{T} \sqrt{\lambda_t}}
\end{equation}

If the stock starts at $N_0$ and ends around $R$ at $t=L$, then $\sum_{t=1}^{K'}(N_0-\lambda_t)\sim \frac{R+N_0}{2}K'$. Let $K'\sim K^*\sim K$ and take $\gamma_{\text{disc}}=1$, then
\begin{equation}
	E_{K}\sim \frac{R+N_0}{2}K
\end{equation}
Now
\begin{equation}
	\begin{split}
		\sum_{t=a}^b\sqrt{\lambda t}&\approx \frac{2\sqrt{\lambda}}{3}(b^\frac{3}{2}-a^\frac{3}{2}),\\
		\sum_{t=a}^b\lambda t& =\lambda \frac{(b-a+1)(a+b)}{2}
	\end{split}
\end{equation}

\begin{equation}
	\sum_{t=K}^{T}\sqrt{\lambda_t}\sim \frac{2\sqrt{\lambda}}{3}(T^\frac{3}{2}-K^\frac{3}{2})
\end{equation}

\begin{equation}
	\frac{\mathbb{E}[C|D,I]|_{\pi = \pi^*} }{\mathbb{E}[C|D,I]|_{\pi = \pi'}}\bigg|_{R\sim 0}\sim \frac{\eta+\frac{4r}{r+1}}{\eta+1+r}
\end{equation}
where
\begin{equation}
	\eta = \frac{12N_0K}{m\sqrt{\lambda}(T^\frac{3}{2}-K^\frac{3}{2})}
\end{equation}
Similarly


\begin{equation}
	\begin{split}
		\frac{\mathbb{E}[C|D,I]|_{\pi = \pi^*} }{\mathbb{E}[C|D,I]|_{\pi = \pi'}}\bigg|_{R\gg 0}&\sim \frac{\frac{R+N_0}{2}K+m\frac{r}{r+1}\frac{2\sqrt{\lambda}}{3}(T^\frac{3}{2}-K^\frac{3}{2})}{\frac{R+N_0}{2}K+R(T-K)}\\
		& = \frac{\eta'+\frac{r}{r+1}}{\eta'+\eta''}\\
	\end{split}
\end{equation}

\begin{equation}
	\eta' = \frac{\frac{R+N_0}{2}K}{m\frac{2\sqrt{\lambda}}{3}(T^\frac{3}{2}-K^\frac{3}{2})}
\end{equation}

\begin{equation}
	\eta'' = \frac{R(T-K)}{m\frac{2\sqrt{\lambda}}{3}(T^\frac{3}{2}-K^\frac{3}{2})}
\end{equation}

======================






\begin{axiom}[Ideal conditions]
	Ideal conditions are defined by
	\begin{enumerate}
		\item there are no legacy decisions, so $\upsilon_t=0$ for $t\in [1,L-1]$,
		\item $N_0$ is such that $K'\sim L$.
		\item $\lambda_t=t\lambda$
	\end{enumerate}
\end{axiom}

\begin{equation}
	\begin{split}
		\lim\limits_{R\rightarrow 0} \mathbb{E}[C'|D,I] & \simeq E_L+\sum_{t=L}^{\infty} \gamma_{\text{disc}}^{t-1}\frac{h_t\lambda_t}{2}\bigg(1+\frac{c_t}{h_t}\bigg)  
		\frac{e^{\frac{m}{\sqrt{\lambda_t}}}-1}{e^{\frac{m}{\sqrt{\lambda_t}}}+1},\\
		\lim\limits_{R\rightarrow \infty} \mathbb{E}[C'|D,I] & \simeq E_L+\sum_{t=L}^{\infty} \gamma_{\text{disc}}^{t-1} 
		h_tR.\\
	\end{split}
\end{equation}






Assuming constant $h,c$, that $E_L$ can be neglected in relative magnitude to the sums over infinity and using that \begin{equation}
	1\leq e^{\frac{m}{\sqrt{\lambda_t}}}\lesssim 1.5 \Rightarrow  e^{\frac{m}{\sqrt{\lambda_t}}}\approx k
\end{equation}
the limit of $R\sim 0$ yields
\begin{equation}
	\begin{split}
		\frac{\mathbb{E}[C^*|D,I]}{\mathbb{E}[C'|D,I]}\bigg|_{R\sim 0} 
		&\approx 2 \frac{\frac{k-1}{k\frac{h}{c} + 1}}{\big(1 + \frac{1}{\frac{h}{c}}\big)\frac{k-1}{1+k}} \frac{\sum_{t=L}^{\infty} \gamma_{\text{disc}}^{t-1} \lambda_t}{\sum_{t=L}^{\infty} \gamma_{\text{disc}}^{t-1} \lambda_t} \\
		&= \frac{2(1+k)}{\big(1 + \frac{1}{\frac{h}{c}}\big)\big(k\frac{h}{c} + 1\big)} \\
		&\simeq \frac{4}{2 + \frac{h}{c} + \frac{c}{h}}
	\end{split}
\end{equation}
where for the last equality it was used that $k\simeq 1$. In the limit of $R\gg 0$
\begin{equation}
	\begin{split}
		\frac{\mathbb{E}[C^*|D,I] }{\mathbb{E}[C'|D,I]}\bigg|_{R\gg 0} &\simeq \frac{\sum_{t=L}^{\infty} \gamma_{\text{disc}}^{t-1} \lambda_th_t\frac{e^{\frac{m}{\sqrt{\lambda_t}}}-1}{e^{\frac{m}{\sqrt{\lambda_t}}}\frac{h_t}{c_t}+1}}{\sum_{t=L}^{\infty} \gamma_{\text{disc}}^{t-1}h_t R} \\
		&=\frac{1}{\frac{h}{c}+1} \frac{m}{R}\frac{\sum_{t=L}^{\infty} \gamma_{\text{disc}}^{t-1} \sqrt{\lambda_t}}{\sum_{t=L}^{\infty} \gamma_{\text{disc}}^{t-1}} \\
	\end{split}
\end{equation}
By definition
\begin{equation}
	\frac{m}{R}\frac{\sum_{t=L}^{\infty} \gamma_{\text{disc}}^{t-1} \sqrt{\lambda_t}}{\sum_{t=L}^{\infty} \gamma_{\text{disc}}^{t-1}} = 1 
\end{equation}
since $0\leq \text{PER}\leq 1$. Therefore
\begin{equation}
	\lim\limits_{R\rightarrow \infty}\frac{\mathbb{E}[C^*|D,I] }{\mathbb{E}[C'|D,I]} \simeq \frac{1}{1+\frac{h}{c}}.
\end{equation}