\section{Poisson Distribution}

\begin{equation}
	p(\zeta\leq k|\lambda) = e^{-\lambda}\sum_{j=0}^k\frac{\lambda^j}{j!}
\end{equation}

\begin{equation}
	\Gamma(s,x) = (s-1)!e^{-x}\sum_{j=0}^{s-1}\frac{\lambda^j}{j!}
\end{equation}
\begin{equation}
	\Gamma(s)= (s-1)!
\end{equation}
hence
\begin{equation}
	p(x\leq s|\lambda)=\frac{\Gamma(s+1,x)}{\Gamma(s+1)}
\end{equation}

Similarly
\begin{equation}
	\begin{split}
		\mathbb{E}[\zeta|\zeta\leq k,\lambda] &= e^{-\lambda}\sum_{j=0}^kj\frac{\lambda^j}{j!}\\
		& = e^{-\lambda}\sum_{j=0}^{k}\frac{\lambda^{j}}{(j-1)!}\\
		& = \lambda e^{-\lambda}\sum_{j=0}^{k-1}\frac{\lambda^{j}}{j!}\\
		& =\lambda \frac{\Gamma(s,x)}{\Gamma(s)}
	\end{split}
\end{equation}
