\section{Minimization of Expected Cost}
\label{app:deriv}
With the cost function
\begin{equation}
	C = \sum_{t=1}^{\infty}\gamma^{t}(k^\text{sc}_{t}N_{t}^{(+)}+k_{t}^\text{uv}N_{t}^{(-)})
\end{equation}
the derivation proceeds analogously to that of appendix \ref{app:deriva}, resulting again in the criterion $\psi_j=0$, however, now with
\begin{equation}
	\psi_t\equiv k^\text{sc}_{t}p(N_t\geq 0|D,I)+k_{t}^\text{uv}(\mathbb{E}[s_t|N_{t}\geq 0,D,I]-\mathbb{E}[s_t|D,I]),
\end{equation} 
and
\begin{equation}
	\begin{split}
		\sum_{s_1,s_2,\dots}s_{t}1_{N_{t}\geq 0}p(s_1,s_{2},\dots|D,I)&=\mathbb{E}[s_t|N_{t}\geq 0,D,I],\\
		\sum_{s_1,s_2,\dots}s_{t}p(s_1,s_{2},\dots|D,I)&=\mathbb{E}[s_t|D,I].\\
	\end{split}
\end{equation}
The resulting optimal decision rules are
\begin{equation}
	\frac{p(N_t^*\geq 0|D,I)}{\mathbb{E}[s_t|D,I]-\mathbb{E}[s_t|N_t^*\geq 0,D,I]}=\frac{k_{t}^\text{uv}}{k^\text{sc}_{t}}.
\end{equation}
