\section{Policy Efficiency Ratio}
\label{app:cer}
The expected cost assuming conditional independence between $\zeta_t$
\begin{equation}
	\begin{split}
		\mathbb{E}[C|D,I] &= \sum_{t=1}^{\infty}\sum_{\zeta_t=0}^\infty \gamma_{\text{disc}}^{t} \left( h_t 1_{N_t> 0} + c_t (1_{N_t> 0}-1) \right)N_tp(\zeta_t| D, I)\\
		&= \sum_{t=1}^{\infty}\sum_{\zeta_t=0}^\infty \gamma_{\text{disc}}^{t} \bigg( 
		(h_t+c_t)(N_0 + \upsilon_t)1_{N_t> 0}\\
		&\qquad\qquad\qquad\quad-(h_t+c_t) 1_{N_t> 0}\zeta_t
		- c_t(N_0 + \upsilon_t)+c_t\zeta_t\bigg)p(\zeta_t| D, I).
	\end{split}
\end{equation}
the sums over $\zeta$ can be written
\begin{equation}
	\begin{split}
		\sum_{\zeta_t=0}^\infty1_{N_t> 0}p(\zeta_t| D, I) & = \sum_{\zeta_t=0}^{N_0+\upsilon_t} p(\zeta_t| D, I)\\
		&= \frac{\Gamma(N_0+\upsilon_t+1,\lambda_t)}{\Gamma(N_0+\upsilon_t+1)},\\
		\sum_{\zeta_t=0}^\infty1_{N_t> 0}\zeta_tp(\zeta_t| D, I) & = \sum_{\zeta_t=0}^{N_0+\upsilon_t} \zeta_t p(\zeta_t| D, I)\\
		& = \lambda_t \frac{\Gamma(N_0+\upsilon_t,\lambda_t)}{\Gamma(N_0+\upsilon_t)},\\
		\sum_{\zeta_t=0}^\infty\zeta_tp(\zeta_t| D, I) & = \lambda_t,\\
		\sum_{\zeta_t=0}^\infty p(\zeta_t| D, I) & = 1.\\
	\end{split}
\end{equation}
The gamma functions are approximated viz~\cite{bartmann1992inventory}
\begin{equation}
	\frac{\Gamma(x,y)}{\Gamma(x)}\simeq \frac{1}{1+e^{-\frac{m}{\sqrt{y}}(x-y)}}
\end{equation}
with $m\simeq 1.8$. This means
\begin{equation}
	\begin{split}
		\sum_{\zeta_t=0}^\infty1_{N_t> 0}p(\zeta_t| D, I) & \simeq \frac{1}{1+e^{-\frac{m}{\sqrt{\lambda_t}}(N_0+\upsilon_t+1-\lambda_t)}}\\
		\sum_{\zeta_t=0}^\infty1_{N_t> 0}\zeta_tp(\zeta_t| D, I) & \simeq \lambda_t\frac{1}{1+e^{-\frac{m}{\sqrt{\lambda_t}}(N_0+\upsilon_t-\lambda_t)}}\\
	\end{split}
\end{equation}
This means
\begin{equation}
	\begin{split}
		\mathbb{E}[C|D,I] &\simeq  \sum_{t=1}^{\infty} \gamma_{\text{disc}}^{t} \bigg( 
		(h_t+c_t)\bigg[\frac{N_0 + \upsilon_t}{1+e^{-\frac{m}{\sqrt{\lambda_t}}(N_0+\upsilon_t+1-\lambda_t)}}- \frac{\lambda_t}{1+e^{-\frac{m}{\sqrt{\lambda_t}}(N_0+\upsilon_t-\lambda_t)}}\bigg]\\
		&\qquad\qquad\qquad
		- c_t(N_0 + \upsilon_t-\lambda_t)\bigg)\\
	\end{split}
\end{equation}

No decisions can be implemented during the lead time, meaning
\begin{equation}
	\begin{split}
		\mathbb{E}[C|D,I] &\simeq E_L+\sum_{t=L}^{\infty} \gamma_{\text{disc}}^{t} \bigg( 
		(h_t+c_t)\bigg[\frac{N_0 + \upsilon_t}{1+e^{-\frac{m}{\sqrt{\lambda_t}}(N_0+\upsilon_t+1-\lambda_t)}}- \frac{\lambda_t}{1+e^{-\frac{m}{\sqrt{\lambda_t}}(N_0+\upsilon_t-\lambda_t)}}\bigg]\\
		&\qquad\qquad\qquad
		- c_t(N_0 + \upsilon_t-\lambda_t)\bigg)\\
	\end{split}
\end{equation}
where
\begin{equation}
	\begin{split}
		E_L\equiv \sum_{t=1}^{L-1} \gamma_{\text{disc}}^{t} \bigg( 
		\frac{N_0(h_t+c_t)}{1+e^{-\frac{m}{\sqrt{\lambda_t}}(N_0+1-\lambda_t)}}- \frac{\lambda_t(h_t+c_t)}{1+e^{-\frac{m}{\sqrt{\lambda_t}}(N_0-\lambda_t)}}- \frac{c_t}{h_t}(N_0-\lambda_t)\bigg)
	\end{split}
\end{equation}


\subsection{Optimal Expected Cost}

\begin{equation}
	\frac{c_t}{c_t+h_t}1_{t\geq L}\simeq\frac{1}{1+e^{-\frac{m}{\sqrt{\lambda_t}}(N_0+\upsilon_t+1-\lambda_t)}}\\
\end{equation}

\begin{equation}
	\frac{c_t}{h_t}1_{t\geq L}\simeq e^{\frac{m}{\sqrt{\lambda_t}}(N_0+\upsilon_t+1-\lambda_t)}\\
\end{equation}

\begin{equation}
	\upsilon_t\simeq 1_{t\geq L}(\lambda_t-N_0-1+\frac{\sqrt{\lambda_t}}{m}\ln\frac{c_t}{h_t}) 
\end{equation}

This means

\begin{equation}
	\begin{split}
		\mathbb{E}[C^*|D,I] &\simeq E_L+ \sum_{t=L}^{\infty} \gamma_{\text{disc}}^{t} \bigg( 
		c_t(N_0 + \upsilon_t)- \lambda_tc_t\frac{c_t+h_t}{c_t+e^{\frac{m}{\sqrt{\lambda_t}}}h_t}- c_t(N_0 + \upsilon_t-\lambda_t)\bigg)\\
		&= E_L+\sum_{t=L}^{\infty} \gamma_{\text{disc}}^{t} \lambda_th_t\frac{e^{\frac{m}{\sqrt{\lambda_t}}}-1}{e^{\frac{m}{\sqrt{\lambda_t}}}\frac{h_t}{c_t}+1}\\
	\end{split}
\end{equation}

\subsection{Baseline Expected Cost}

\begin{equation}
	\upsilon_t= 1_{t\geq L}(\lambda_t-N_0)
\end{equation}

\begin{equation}
	\begin{split}
		\mathbb{E}[C'|D,I] &\simeq E_L+\sum_{t=L}^{\infty} \gamma_{\text{disc}}^{t} h_t\lambda_t 
		\bigg(1+\frac{1}{\frac{h_t}{c_t}}\bigg)\bigg[\frac{1}{1+e^{-\frac{m}{\sqrt{\lambda_t}}}}- \frac{1}{2}\bigg]\\
		&= E_L+\sum_{t=L}^{\infty} \gamma_{\text{disc}}^{t} \frac{h_t\lambda_t}{2} 
		\bigg(1+\frac{1}{\frac{h_t}{c_t}}\bigg)\frac{e^{\frac{m}{\sqrt{\lambda_t}}}-1}{1+e^{\frac{m}{\sqrt{\lambda_t}}}}\\
	\end{split}
\end{equation}


\subsection{Policy Efficiency Ratio}

\begin{equation}
	\frac{\mathbb{E}[C^*|D,I] }{\mathbb{E}[C'|D,I]}\simeq \frac{E_L+\sum_{t=L}^{\infty} \gamma_{\text{disc}}^{t} \lambda_th_t\frac{e^{\frac{m}{\sqrt{\lambda_t}}}-1}{e^{\frac{m}{\sqrt{\lambda_t}}}\frac{h_t}{c_t}+1}}{E_L+\sum_{t=L}^{\infty} \gamma_{\text{disc}}^{t} \frac{h_t\lambda_t}{2} 
		(1+\frac{1}{\frac{h_t}{c_t}})\frac{e^{\frac{m}{\sqrt{\lambda_t}}}-1}{1+e^{\frac{m}{\sqrt{\lambda_t}}}}}
\end{equation}
Assuming constant $h,c$, that $E_L$ can be neglected in relative magnitude to the sums over infinity and using that \begin{equation}
	1\leq e^{\frac{m}{\sqrt{\lambda_t}}}\lesssim 1.5 \Rightarrow  e^{\frac{m}{\sqrt{\lambda_t}}}\approx k
\end{equation}
yields
\begin{equation}
	\begin{split}
		\frac{\mathbb{E}[C^*|D,I] }{\mathbb{E}[C'|D,I]}&\approx2 \frac{\frac{k-1}{k\frac{h_t}{c_t}+1}}{(1+\frac{1}{\frac{h_t}{c_t}})\frac{k-1}{1+k}}\frac{\sum_{t=L}^{\infty} \gamma_{\text{disc}}^{t} \lambda_t}{\sum_{t=L}^{\infty} \gamma_{\text{disc}}^{t} \lambda_t}\\
		&= \frac{2(1+k)}{(1+\frac{1}{\frac{h_t}{c_t}})(k\frac{h_t}{c_t}+1)}\\
		&\simeq \frac{4}{2+\frac{h_t}{c_t}+\frac{c_t}{h_t}}\\
	\end{split}
\end{equation}
where for the last equality it was used that $k\simeq 1$. 